coq_session/proc_occurs.v
@@ -6,79 +6,96 @@ Set Implicit Arguments.
 Unset Strict Implicit.
 Unset Printing Implicit Defensive.
 
-Inductive proc_occurs : dyn_ctx -> proc -> cvar -> nat -> Prop :=
-| proc_occurs_exp Θ m i j :
-  dyn_occurs Θ nil nil m (IO Unit) i j ->
-  proc_occurs Θ ⟨ m ⟩ i j
-| proc_occurs_par Θ1 Θ2 Θ p q i j1 j2 :
-  Θ1 ∘ Θ2 => Θ ->
-  proc_occurs Θ1 p i j1 ->
-  proc_occurs Θ2 q i j2 ->
-  proc_occurs Θ (p ∣ q) i (j1 + j2)
-| proc_occurs_scope Θ p r1 r2 A i j :
-  r1 = ~~r2 ->
-  proc_occurs (Ch r1 (term_cren A (+1)) :L Ch r2 A :L Θ) p i.+2 j ->
-  proc_occurs Θ (ν.p) i j
-where "Θ ⊢ p" := (proc_type Θ p).
+Fixpoint proc_occurs (i : cvar) (p : proc) : nat :=
+  match p with
+  | ⟨ m ⟩ => dyn_occurs i m
+  | p ∣ q => proc_occurs i p + proc_occurs i q
+  | ν.p => proc_occurs i.+2 p
+  end.
 
 Lemma proc_type_occurs0 Θ p i :
-  Θ ⊢ p -> cvar_pos Θ i false -> proc_occurs Θ p i 0.
+  Θ ⊢ p -> cvar_pos Θ i false -> proc_occurs i p = 0.
 Proof with eauto using cvar_pos.
-  move=>ty. elim: ty i=>{Θ p}.
+  move=>ty. elim: ty i=>//={Θ p}.
   { move=>Θ m tym i pos.
-    constructor. apply: dyn_type_occurs0... }
+    apply: dyn_type_occurs0... }
   { move=>Θ1 Θ2 Θ p q mrg typ ihp tyq ihq i pos.
     have[pos1 pos2]:=cvar_pos_split_false mrg pos.
-    replace 0 with (0 + 0) by eauto.
-    econstructor... }
+    rewrite ihp... }
   { move=>Θ p r1 r2 A xor typ ihp i pos.
-    econstructor... }
+    rewrite ihp... }
 Qed.
 
 Lemma proc_type_occurs1 Θ p i :
-  Θ ⊢ p -> cvar_pos Θ i true -> proc_occurs Θ p i 1.
+  Θ ⊢ p -> cvar_pos Θ i true -> proc_occurs i p = 1.
 Proof with eauto using cvar_pos, proc_occurs, proc_type_occurs0.
-  move=>ty. elim: ty i=>{Θ p}.
+  move=>ty. elim: ty i=>//={Θ p}.
   { move=>Θ m tym i pos.
-    constructor. apply: dyn_type_occurs1... }
+    apply: dyn_type_occurs1... }
   { move=>Θ1 Θ2 Θ p q mrg typ ihp tyq ihq i pos.
     have[[pos1 pos2]|[pos1 pos2]]:=cvar_pos_split_true mrg pos.
-    { replace 1 with (0 + 1) by eauto... }
-    { replace 1 with (1 + 0) by eauto... } }
+    { erewrite ihq...
+      erewrite proc_type_occurs0... }
+    { erewrite ihp... } }
   { move=>Θ p r1 r2 A xor typ ihp i pos.
-    econstructor... }
-Qed.
-
-Lemma proc_occurs_pos0 Θ p i :
-  proc_occurs Θ p i 0 -> cvar_pos Θ i false.
-Proof with eauto using cvar_pos.
-  move e:(0)=>j ty. elim: ty e=>{Θ p i j}.
-  { move=>Θ m i j ty e. subst.
-    apply: dyn_occurs_pos0... }
-  { move=>Θ1 Θ2 Θ p q i j1 j2 mrg typ ihp tyq ihq e.
-    destruct j1; destruct j2; inv e.
-    apply: cvar_pos_merge_false... }
-  { move=>Θ p r1 r2 A i j e1 typ ihp e2. subst.
-    have{}ihp:=ihp erefl.
-    inv ihp. inv H3... }
+    rewrite ihp... }
 Qed.
 
 Lemma proc_occurs_iren Θ p i ξ :
-  Θ ⊢ proc_cren p ξ -> iren i ξ -> proc_occurs Θ (proc_cren p ξ) i 0.
+  Θ ⊢ proc_cren p ξ -> iren i ξ -> proc_occurs i (proc_cren p ξ) = 0.
 Proof with eauto using proc_occurs.
   move e:(proc_cren p ξ)=>x ty.
-  elim: ty p ξ e i=>{Θ x}.
+  elim: ty p ξ e i=>//={Θ x}.
   { move=>Θ m tym p ξ e i h.
     destruct p; inv e.
-    constructor.
     apply: dyn_occurs_iren... }
   { move=>Θ1 Θ2 Θ p q mrg typ ihp tyq ihq x ξ e i h.
     destruct x; inv e.
-    replace 0 with (0 + 0) by eauto... }
+    erewrite ihp... }
   { move=>Θ p r1 r2 A e1 typ ihp x ξ e i h.
     destruct x; inv e.
-    econstructor...
     apply: ihp...
     apply: iren_upren.
     by apply: iren_upren. }
+Qed.
+
+Lemma cren_id_up2 i j ξ :
+  (forall x, (x == i) = false → (x == j) = false → ξ x = x) ->
+  (forall x, (x == i.+2) = false → (x == j.+2) = false → upren (upren ξ) x = x).
+Proof.
+  move=>h [|[|x]]//=.
+  move=>e1 e2.
+  f_equal.
+  f_equal.
+  apply: h; lia.
+Qed.
+
+Lemma proc_occurs_cren_id Θ p i j ξ :
+  Θ ⊢ proc_cren p ξ ->
+  proc_occurs i p = 0 ->
+  proc_occurs j p = 0 ->
+  (forall x, x == i = false -> x == j = false -> ξ x = x) ->
+  Θ ⊢ p.
+Proof with eauto using proc_type.
+  move e:(proc_cren p ξ)=>p' ty.
+  elim: ty p ξ e i j=>{Θ p'}.
+  { move=>Θ m tym p ξ e i j oc1 oc2 h.
+    destruct p; inv e. simpl in oc1. simpl in oc2.
+    constructor.
+    apply: dyn_occurs_cren_id.
+    eauto.
+    apply: oc1.
+    apply: oc2.
+    eauto. }
+  { move=>Θ1 Θ2 Θ p q mrg typ ihp tyq ihq p0 ξ e i j oc1 oc2 h.
+    destruct p0; inv e. simpl in oc1. simpl in oc2.
+    move: oc1. case_eq (proc_occurs i p0_1); case_eq (proc_occurs i p0_2)=>//=e1 e2 _.
+    move: oc2. case_eq (proc_occurs j p0_1); case_eq (proc_occurs j p0_2)=>//=e3 e4 _.
+    have{}ihp:=ihp _ _ erefl _ _ e2 e4 h.
+    have{}ihq:=ihq _ _ erefl _ _ e1 e3 h.
+    econstructor... }
+  { move=>Θ p r1 r2 A e0 typ ihp p0 ξ e i j oc1 oc2 h.
+    destruct p0; inv e. simpl in oc1. simpl in oc2.
+    have{}ihp:=ihp _ _ erefl _ _ oc1 oc2 (cren_id_up2 h).
+    econstructor... }
 Qed.
