coq_session/proc_step.v
@@ -1,6 +1,6 @@
 From mathcomp Require Import ssreflect ssrbool eqtype ssrnat seq.
 From Coq Require Import ssrfun Classical Utf8.
-Require Export AutosubstSsr ARS proc_cren.
+Require Export AutosubstSsr ARS proc_cren proc_occurs.
 
 Set Implicit Arguments.
 Unset Strict Implicit.
@@ -11,30 +11,21 @@ Inductive proc_congr0 : proc -> proc -> Prop :=
   proc_congr0 (p ∣ q) (q ∣ p)
 | proc_congr0_assoc o p q :
   proc_congr0 (o ∣ (p ∣ q)) ((o ∣ p) ∣ q)
-| proc_congr0_associ o p q :
-  proc_congr0 ((o ∣ p) ∣ q) (o ∣ (p ∣ q)) 
-| proc_congr0_scope p (q : proc) :
+| proc_congr0_extrude p (q : proc) :
   proc_congr0 ((ν.p) ∣ q) (ν.(p ∣ proc_cren q (+2)))
-| proc_congr0_scopei p (q : proc) :
-  proc_congr0 (ν.(p ∣ proc_cren q (+2))) ((ν.p) ∣ q) 
+| proc_congr0_contract p (q : proc) :
+  proc_occurs 0 q = 0 ->
+  proc_occurs 1 q = 0 ->
+  proc_congr0 (ν.(p ∣ q)) ((ν.p) ∣ proc_cren q (-2)) 
 | proc_congr0_par p p' q q' :
   proc_congr0 p p' ->
   proc_congr0 q q' ->
   proc_congr0 (p ∣ q) (p' ∣ q')
-| proc_congr0_pari p p' q q' :
-  proc_congr0 p p' ->
-  proc_congr0 q q' ->
-  proc_congr0 (p' ∣ q') (p ∣ q) 
 | proc_congr0_nu p p' :
   proc_congr0 p p' ->
   proc_congr0 (ν.p) (ν.p')
-| proc_congr0_nui p p' :
-  proc_congr0 p p' ->
-  proc_congr0 (ν.p') (ν.p)
 | proc_congr0_end p :
-  proc_congr0 (p ∣ ⟨ Return II ⟩) p
-| proc_congr0_endi p :
-  proc_congr0 p (p ∣ ⟨ Return II ⟩).
+  proc_congr0 (p ∣ ⟨ Return II ⟩) p.
 Notation "p ≡ q" := (conv proc_congr0 p q) (at level 50).
 
 Reserved Notation "p ≈>> q" (at level 50).
@@ -52,18 +43,18 @@ Inductive proc_step : proc -> proc -> Prop :=
   n' = term_cren n (+2) ->
   ⟨ Bind (Fork A m) n ⟩ ≈>> ν.(⟨ n'.[CVar 0/] ⟩ ∣ ⟨ m'.[CVar 1/] ⟩)
 | proc_step_com0 m n1 n2 :
-  ν.(⟨ Bind (App (Send0 (CVar 0)) m) n1 ⟩ ∣ ⟨ Bind (Recv0 (CVar 1)) n2 ⟩) ≈>>
+  ν.(⟨ Bind (App0 (Send0 (CVar 0)) m) n1 ⟩ ∣ ⟨ Bind (Recv0 (CVar 1)) n2 ⟩) ≈>>
   ν.(⟨ Bind (Return (CVar 0)) n1 ⟩ ∣ ⟨ Bind (Return (Pair0 m (CVar 1) L)) n2 ⟩)
 | proc_step_com0i m n1 n2 :
-  ν.(⟨ Bind (App (Send0 (CVar 1)) m) n1 ⟩ ∣ ⟨ Bind (Recv0 (CVar 0)) n2 ⟩) ≈>>
+  ν.(⟨ Bind (App0 (Send0 (CVar 1)) m) n1 ⟩ ∣ ⟨ Bind (Recv0 (CVar 0)) n2 ⟩) ≈>>
   ν.(⟨ Bind (Return (CVar 1)) n1 ⟩ ∣ ⟨ Bind (Return (Pair0 m (CVar 0) L)) n2 ⟩)
 | proc_step_com1 v n1 n2 :
   dyn_val v ->
-  ν.(⟨ Bind (App (Send1 (CVar 0)) v) n1 ⟩ ∣ ⟨ Bind (Recv1 (CVar 1)) n2 ⟩) ≈>>
+  ν.(⟨ Bind (App1 (Send1 (CVar 0)) v) n1 ⟩ ∣ ⟨ Bind (Recv1 (CVar 1)) n2 ⟩) ≈>>
   ν.(⟨ Bind (Return (CVar 0)) n1 ⟩ ∣ ⟨ Bind (Return (Pair1 v (CVar 1) L)) n2 ⟩)
 | proc_step_com1i v n1 n2 :
   dyn_val v ->
-  ν.(⟨ Bind (App (Send1 (CVar 1)) v) n1 ⟩ ∣ ⟨ Bind (Recv1 (CVar 0)) n2 ⟩) ≈>>
+  ν.(⟨ Bind (App1 (Send1 (CVar 1)) v) n1 ⟩ ∣ ⟨ Bind (Recv1 (CVar 0)) n2 ⟩) ≈>>
   ν.(⟨ Bind (Return (CVar 1)) n1 ⟩ ∣ ⟨ Bind (Return (Pair1 v (CVar 0) L)) n2 ⟩)
 | proc_step_end m m' n n' :
   m' = term_cren m (-2) ->
