coq_session/sta_cren.v
@@ -6,38 +6,6 @@ Set Implicit Arguments.
 Unset Strict Implicit.
 Unset Printing Implicit Defensive.
 
-Inductive sta_agree_cren : (cvar -> cvar) -> sta_ctx -> sta_ctx -> Prop :=
-| sta_agree_cren_nil ξ :
-  sta_agree_cren ξ nil nil
-| sta_agree_cren_cons Γ Γ' ξ m m' s :
-  m' = term_cren m ξ ->
-  Γ ⊢ m : Sort s ->
-  sta_agree_cren ξ Γ Γ' ->
-  sta_agree_cren ξ (m :: Γ) (m' :: Γ').
-
-Lemma sta_agree_cren_size Γ Γ' ξ :
-  sta_agree_cren ξ Γ Γ' -> size Γ = size Γ'.
-Proof with eauto.
-  elim=>{Γ Γ' ξ}...
-  move=>Γ Γ' ξ m m' s e1 tym agr e2=>//=.
-  by rewrite e2.
-Qed.
-
-Lemma sta_agree_cren_has Γ Γ' ξ x A :
-  sta_agree_cren ξ Γ Γ' ->
-  sta_has Γ x A ->
-  sta_has Γ' x (term_cren A ξ).
-Proof with eauto.
-  move=>agr. elim: agr x A=>{Γ Γ' ξ}.
-  { move=>ξ x A shs. inv shs. }
-  { move=>Γ Γ' ξ m m' s e tym agr ih x A shs. subst.
-    inv shs.
-    { rewrite term_cren_ren.
-      constructor. }
-    { rewrite term_cren_ren.
-      constructor... } }
-Qed.
-
 Lemma sta_cren_pstep0 m n ξ : m ≈> n -> term_cren m ξ ≈> n.
 Proof with eauto using sta_pstep. move=>st. elim: st ξ=>//={m n}... Qed.
 
@@ -107,110 +75,525 @@ Proof with eauto using sta_pstep.
     by apply: sta_cren_pstep. }
 Qed.
 
-Lemma sta_crename Γ Γ' m A ξ :
-  Γ ⊢ m : A -> sta_agree_cren ξ Γ Γ' ->
-  Γ' ⊢ term_cren m ξ : term_cren A ξ.
-Proof with eauto using sta_type, sta_agree_cren.
-  move=>ty. move:Γ m A ty Γ' ξ.
-  apply:(@sta_type_mut _ (fun Γ wf => forall Γ' ξ, sta_agree_cren ξ Γ Γ' -> sta_wf Γ')); simpl...
-  { move=>Γ x A wf ih shs Γ' ξ agr.
-    constructor...
-    apply: sta_agree_cren_has... }
-  { move=>Γ A B m s tym ihm Γ' ξ agr.
-    have wf:=sta_type_wf tym. inv wf.
+Lemma sta_crename Γ m A ξ :
+  Γ ⊢ m : A -> Γ ⊢ term_cren m ξ : A.
+Proof with eauto using sta_type, sta0_sta_wf.
+  move=>ty. have{}ty:=sta_sta0_type ty.
+  elim: ty ξ=>//={Γ m A}...
+  { move=>Γ A B s r t/sta0_sta_type tyA ihA/sta0_sta_type tyB ihB ξ.
+    econstructor...
+    apply: sta_ctx_conv.
+    apply: sta_cren_conv0...
+    all: eauto. }
+  { move=>Γ A B s r t/sta0_sta_type tyA ihA/sta0_sta_type tyB ihB ξ.
+    econstructor...
+    apply: sta_ctx_conv.
+    apply: sta_cren_conv0...
+    all: eauto. }
+  { move=>Γ A B m s r/sta0_sta_type tyA ihA/sta0_sta_type tym ihm ξ.
+    have[t tyB]:=sta_valid tym.
     econstructor.
-    apply: ihm.
-    econstructor... }
-  { move=>Γ A B m s tym ihm Γ' ξ agr.
-    have wf:=sta_type_wf tym. inv wf.
-    econstructor.
-    apply: ihm.
-    econstructor... }
-  { move=>Γ A B m n s tym ihm tyn ihn Γ' ξ agr.
-    rewrite term_cren_beta1.
-    apply: sta_app0... }
-  { move=>Γ A B m n s tym ihm tyn ihn Γ' ξ agr.
-    rewrite term_cren_beta1.
-    apply: sta_app1... }
-  { move=>Γ A B m n t tyS ihS tym ihm tyn ihn Γ' ξ agr.
-    apply: sta_pair0...
-    rewrite<-term_cren_beta1... }
-  { move=>Γ A B m n t tyS ihS tym ihm tyn ihn Γ' ξ agr.
-    apply: sta_pair1...
-    rewrite<-term_cren_beta1... }
-  { move=>Γ A B C m n s t tyC ihC tym ihm tyn ihn Γ' ξ agr.
-    have wf:=sta_type_wf tyC. inv wf.
-    have wf:=sta_type_wf tyn. inv wf. inv H3.
-    rewrite term_cren_beta1.
-    apply: sta_letin0...
-    apply: ihC...
-    rewrite<-(term_cren_subst _ (term_csubst_pair0 ξ t)).
-    apply: ihn... }
-  { move=>Γ A B C m n s t tyC ihC tym ihm tyn ihn Γ' ξ agr.
-    have wf:=sta_type_wf tyC. inv wf.
-    have wf:=sta_type_wf tyn. inv wf. inv H3.
-    rewrite term_cren_beta1.
-    apply: sta_letin1...
-    apply: ihC...
-    rewrite<-(term_cren_subst _ (term_csubst_pair1 ξ t)).
-    apply: ihn... }
-  { move=>Γ A m tym ihm Γ' ξ agr.
-    have wf:=sta_type_wf tym. inv wf.
+    apply: sta_conv_pi0.
+    apply: sta_cren_conv0.
+    apply: ξ.
+    eauto.
+    eauto.
     constructor.
-    rewrite<-term_cren_ren.
-    apply: ihm... }
-  { move=>Γ A m n1 n2 s tyA ihA tym ihm tyn1 ihn1 tyn2 ihn2 Γ' ξ
-           agr.
-    rewrite term_cren_beta1.
-    apply: sta_ifte...
-    replace TT with (term_cren TT ξ) by eauto.
-    rewrite<-term_cren_beta1...
-    replace FF with (term_cren FF ξ) by eauto.
-    rewrite<-term_cren_beta1... }
-  { move=>Γ m n A B s tyB ihB tym ihm tyn ihn Γ' ξ agr.
-    have wf:=sta_type_wf tyn. inv wf.
-    apply: sta_bind...
-    rewrite<-term_cren_ren... }
-  { move=>Γ r A B tyB ihB Γ' ξ agr.
-    have wf:=sta_type_wf tyB. inv wf.
-    apply: sta_act0. apply: ihB... }
-  { move=>Γ r A B tyB ihB Γ' ξ agr.
-    have wf:=sta_type_wf tyB. inv wf.
-    apply: sta_act1. apply: ihB... }
-  { move=>Γ r x A wf ih tyA ihA Γ' ξ agr.
-    rewrite term_cren_ren.
-    rewrite (sta_agree_cren_size agr).
-    apply: sta_cvar... }
-  { move=>Γ m A tym ihm Γ' ξ agr.
-    have wf:=sta_type_wf tym. inv wf.
-    constructor... }
-  { move=>Γ A B m s eq tym ihm tyB ihB Γ' ξ agr.
-    apply: sta_conv.
-    apply: sta_cren_conv...
-    apply: ihm...
-    apply: ihB... }
-  { move=>Γ' ξ agr. inv agr. constructor. }
-  { move=>Γ A s wf ih tyA ihA Γ' ξ agr. inv agr.
+    apply: sta_ctx_conv.
+    apply: sta_cren_conv0...
+    eauto.
+    eauto.
     econstructor... }
+  { move=>Γ A B m s r/sta0_sta_type tyA ihA/sta0_sta_type tym ihm ξ.
+    have[t tyB]:=sta_valid tym.
+    econstructor.
+    apply: sta_conv_pi1.
+    apply: sta_cren_conv0.
+    apply: ξ.
+    eauto.
+    eauto.
+    constructor.
+    apply: sta_ctx_conv.
+    apply: sta_cren_conv0...
+    eauto.
+    eauto.
+    econstructor... }
+  { move=>Γ A B m n s/sta0_sta_type tym ihm/sta0_sta_type tyn ihn ξ.
+    have[r tyPi0]:=sta_valid tym.
+    have[t[tyB/sort_inj e]]:=sta_pi0_inv tyPi0. subst.
+    have/=tyBn:=sta_subst tyB tyn.
+    apply: sta_conv.
+    apply: sta_conv_beta.
+    apply: sta_cren_conv0...
+    econstructor...
+    eauto. }
+  { move=>Γ A B m n s/sta0_sta_type tym ihm/sta0_sta_type tyn ihn ξ.
+    have[r tyPi1]:=sta_valid tym.
+    have[t[tyB/sort_inj e]]:=sta_pi1_inv tyPi1. subst.
+    have/=tyBn:=sta_subst tyB tyn.
+    apply: sta_conv.
+    apply: sta_conv_beta.
+    apply: sta_cren_conv0...
+    econstructor...
+    eauto. }
+  { move=>Γ A B s r t ord/sta0_sta_type tyA ihA/sta0_sta_type tyB ihB ξ.
+    econstructor...
+    apply: sta_ctx_conv.
+    apply: sta_cren_conv0...
+    all: eauto. }
+  { move=>Γ A B s r t ord1 ord2/sta0_sta_type tyA ihA/sta0_sta_type tyB ihB ξ.
+    econstructor.
+    apply: ord1.
+    apply: ord2.
+    eauto.
+    apply: sta_ctx_conv.
+    apply: sta_cren_conv0...
+    all: eauto. }
+  { move=>Γ A B m n t/sta0_sta_type tyS ihS/sta0_sta_type tym ihm/sta0_sta_type tyn ihn ξ.
+    have[s[r[ord[tyA[tyB _]]]]]:=sta_sig0_inv tyS.
+    have/=tyBm:=sta_subst tyB (ihm ξ).
+    econstructor...
+    apply: sta_conv.
+    apply: sta_conv_beta.
+    apply: conv_sym.
+    apply: sta_cren_conv0...
+    eauto.
+    eauto. }
+  { move=>Γ A B m n t/sta0_sta_type tyS ihS/sta0_sta_type tym ihm/sta0_sta_type tyn ihn ξ.
+    have[s[r[ord1[ord2[tyA[tyB _]]]]]]:=sta_sig1_inv tyS.
+    have/=tyBm:=sta_subst tyB (ihm ξ).
+    econstructor...
+    apply: sta_conv.
+    apply: sta_conv_beta.
+    apply: conv_sym.
+    apply: sta_cren_conv0...
+    eauto.
+    eauto. }
+  { move=>Γ A B C m n s t/sta0_sta_type tyS ihS/sta0_sta_type tym ihm/sta0_sta_type tyn ihn ξ.
+    have wf:=sta_type_wf tyS. inv wf.
+    have[s1[r[ord[tyA[tyB/sort_inj e]]]]]:=sta_sig0_inv H2. subst.
+    have eq: (term_cren C ξ).[term_cren m ξ/] === C.[m/].
+    apply: conv_trans.
+    apply: sta_conv_beta.
+    apply: sta_cren_conv0...
+    apply: conv_trans.
+    apply: sta_conv_subst.
+    apply: sta_cren_conv0...
+    eauto.
+    apply: sta_conv...
+    econstructor...
+    apply: sta_conv.
+    erewrite<-term_cren_subst.
+    apply: conv_sym.
+    apply: sta_cren_conv0...
+    2:{ apply: ihn. }
+    move=>[|x]/=...
+    have agr:sta_agree_subst (B :: A :: Γ) (Pair0 (Var 1) (Var 0) t .: ren (+2)) (Sig0 A B t :: Γ).
+    { econstructor.
+      replace (ren (+2)) with (ids >> (ren (+1)) >> (ren (+1))) by autosubst.
+      econstructor...
+      econstructor...
+      asimpl.
+      econstructor.
+      replace (Sig0 A.[ren (+2)] B.[ren (0 .: (+3))] t)
+        with (Sig0 A B t).[ren (+2)] by autosubst.
+      replace (Sort t) with (Sort t).[ren (+2)] by eauto.
+      apply: sta_rename...
+      replace (+2) with ((+1) >>> (+1) >>> id) by autosubst.
+      econstructor...
+      econstructor...
+      apply: sta_agree_ren_refl...
+      repeat constructor...
+      replace A.[ren (+2)] with A.[ren (+1)].[ren (+1)] by autosubst.
+      repeat constructor.
+      asimpl.
+      repeat constructor... }
+    have//=:=sta_substitution (ihS ξ) agr.
+    eauto.
+    have//=:=sta_subst tyS tym... }
+  { move=>Γ A B C m n s t/sta0_sta_type tyS ihS/sta0_sta_type tym ihm/sta0_sta_type tyn ihn ξ.
+    have wf:=sta_type_wf tyS. inv wf.
+    have[s1[r[ord1[ord2[tyA[tyB/sort_inj e]]]]]]:=sta_sig1_inv H2. subst.
+    have eq: (term_cren C ξ).[term_cren m ξ/] === C.[m/].
+    apply: conv_trans.
+    apply: sta_conv_beta.
+    apply: sta_cren_conv0...
+    apply: conv_trans.
+    apply: sta_conv_subst.
+    apply: sta_cren_conv0...
+    eauto.
+    apply: sta_conv...
+    apply: sta_letin1...
+    apply: sta_conv.
+    erewrite<-term_cren_subst.
+    apply: conv_sym.
+    apply: sta_cren_conv0...
+    2:{ apply: ihn. }
+    move=>[|x]/=...
+    have agr:sta_agree_subst (B :: A :: Γ) (Pair1 (Var 1) (Var 0) t .: ren (+2)) (Sig1 A B t :: Γ).
+    { econstructor.
+      replace (ren (+2)) with (ids >> (ren (+1)) >> (ren (+1))) by autosubst.
+      econstructor...
+      econstructor...
+      asimpl.
+      econstructor.
+      replace (Sig1 A.[ren (+2)] B.[ren (0 .: (+3))] t)
+        with (Sig1 A B t).[ren (+2)] by autosubst.
+      replace (Sort t) with (Sort t).[ren (+2)] by eauto.
+      apply: sta_rename...
+      replace (+2) with ((+1) >>> (+1) >>> id) by autosubst.
+      econstructor...
+      econstructor...
+      apply: sta_agree_ren_refl...
+      repeat constructor...
+      replace A.[ren (+2)] with A.[ren (+1)].[ren (+1)] by autosubst.
+      repeat constructor.
+      asimpl.
+      repeat constructor... }
+    have//=:=sta_substitution (ihS ξ) agr.
+    eauto.
+    have//=:=sta_subst tyS tym... }
+  { move=>Γ A m s/sta0_sta_type tyA ihA/sta0_sta_type tym ihm ξ.
+    apply: sta_conv.
+    apply: sta_cren_conv0...
+    constructor.
+    apply: sta_ctx_conv.
+    apply: sta_cren_conv0...
+    apply: ihA.
+    apply: sta_conv.
+    apply: sta_conv_subst.
+    apply: conv_sym.
+    apply: sta_cren_conv0...
+    apply: ihm.
+    have//=:=sta_weaken (ihA ξ) tyA...
+    eauto. }
+  { move=>Γ A m n1 n2 s/sta0_sta_type tyA ihA/sta0_sta_type tym ihm
+           /sta0_sta_type tyn1 ihn1/sta0_sta_type tyn2 ihn2 ξ.
+    have wf:=sta_type_wf tym.
+    have eq:(term_cren A ξ).[term_cren m ξ/] === A.[m/].
+    apply: conv_trans.
+    apply: sta_conv_beta.
+    apply: sta_cren_conv0...
+    apply: sta_conv_subst.
+    apply: sta_cren_conv0...
+    apply: sta_conv...
+    econstructor...
+    apply: sta_conv.
+    apply: sta_conv_subst.
+    apply: conv_sym.
+    apply: sta_cren_conv0...
+    eauto.
+    have//=:=sta_subst (ihA ξ) (sta_tt wf)...
+    apply: sta_conv.
+    apply: sta_conv_subst.
+    apply: conv_sym.
+    apply: sta_cren_conv0...
+    eauto.
+    have//=:=sta_subst (ihA ξ) (sta_ff wf)...
+    have//=:=sta_subst tyA tym... }
+  { move=>Γ m n A B s/sta0_sta_type tyB ihB/sta0_sta_type tym ihm/sta0_sta_type tyn ihn ξ.
+    econstructor... }
+  { move=>Γ r A B s/sta0_sta_type tyA ihA/sta0_sta_type tyB ihB ξ.
+    econstructor.
+    apply: sta_ctx_conv.
+    apply: sta_cren_conv0...
+    apply: ihA.
+    apply: ihB. }
+  { move=>Γ r A B s/sta0_sta_type tyA ihA/sta0_sta_type tyB ihB ξ.
+    econstructor.
+    apply: sta_ctx_conv.
+    apply: sta_cren_conv0...
+    apply: ihA.
+    apply: ihB. }
+  { move=>Γ r x A/sta0_sta_wf wf/sta0_sta_type tyA ihA ξ.
+    econstructor... }
+  { move=>Γ A m s/sta0_sta_type tyCh ihCh/sta0_sta_type tym ihm ξ.
+    have[tyA _]:=sta_ch_inv tyCh.
+    apply: sta_conv.
+    apply: sta_conv_io.
+    apply: sta_conv_ch.
+    apply: sta_cren_conv0...
+    econstructor.
+    apply: sta_ctx_conv.
+    apply: sta_conv_ch.
+    apply: sta_cren_conv0...
+    all: eauto.
+    econstructor.
+    econstructor... }
+  { move=>Γ A B m s eq1/sta0_sta_type tym ihm/sta0_sta_type tyB ihB ξ.
+    apply: sta_conv.
+    apply: eq1.
+    all: eauto. }
 Qed.
 
-Lemma sta_ecrename Γ Γ' m m' A A' ξ :
+Lemma sta_ecrename Γ m m' A ξ :
   m' = term_cren m ξ ->
-  A' = term_cren A ξ ->
-  Γ ⊢ m : A -> sta_agree_cren ξ Γ Γ' ->
-  Γ' ⊢ m' : A'.
-Proof. move=>->->. apply: sta_crename. Qed.
+  Γ ⊢ m : A -> Γ ⊢ m' : A.
+Proof. move=>->. apply: sta_crename. Qed.
 
-Lemma sta_crename0 m A ξ :
-  nil ⊢ m : A -> nil ⊢ term_cren m ξ : A.
-Proof with eauto.
-  move=>tym.
-  have[s tyA]:=sta_valid tym.
-  apply: sta_conv.
-  apply: sta_cren_conv0.
-  apply: ξ.
-  eauto.
-  apply: sta_crename...
-  constructor.
-  apply: tyA.
+Ltac sta0_to_sta :=
+  repeat match goal with
+    | [ H : sta0_wf _ |- _ ] => apply sta0_sta_wf in H
+    | [ H : sta0_type _ _ _ |- _ ] => apply sta0_sta_type in H
+    end.
+
+Lemma sta_crename_inv Γ m A ξ :
+  Γ ⊢ term_cren m ξ : A -> Γ ⊢ m : A.
+Proof with eauto using sta_type, sta0_sta_wf.
+  move e:(term_cren m ξ)=>n/sta_sta0_type ty.
+  elim: ty m ξ e=>//={Γ n A}...
+  all: try solve[intros; sta0_to_sta;
+                 match goal with
+                 | [ H : term_cren ?m _ = _ |- _ ] =>
+                     destruct m; inv H; eauto using sta_type, sta_wf
+                 end].
+  { move=>Γ A B s r t tyA ihA tyB ihB m ξ e. sta0_to_sta.
+    destruct m ; inv e.
+    econstructor...
+    apply: sta_ctx_conv.
+    apply: conv_sym.
+    apply: sta_cren_conv0...
+    apply: ihA...
+    eauto. }
+  { move=>Γ A B s r t tyA ihA tyB ihB m ξ e. sta0_to_sta.
+    destruct m ; inv e.
+    econstructor...
+    apply: sta_ctx_conv.
+    apply: conv_sym.
+    apply: sta_cren_conv0...
+    apply: ihA...
+    eauto. }
+  { move=>Γ A B m s r tyA ihA tym ihm m0 ξ e. sta0_to_sta.
+    destruct m0; inv e.
+    have[s0 tyB]:=sta_valid tym.
+    apply: sta_conv.
+    apply: sta_conv_pi0.
+    apply: conv_sym.
+    apply: sta_cren_conv0...
+    eauto.
+    econstructor.
+    apply: sta_ctx_conv.
+    apply: conv_sym.
+    apply: sta_cren_conv0...
+    apply: ihA...
+    apply: ihm...
+    econstructor... }
+  { move=>Γ A B m s r tyA ihA tym ihm m0 ξ e. sta0_to_sta.
+    destruct m0; inv e.
+    have[s0 tyB]:=sta_valid tym.
+    apply: sta_conv.
+    apply: sta_conv_pi1.
+    apply: conv_sym.
+    apply: sta_cren_conv0...
+    eauto.
+    econstructor.
+    apply: sta_ctx_conv.
+    apply: conv_sym.
+    apply: sta_cren_conv0...
+    apply: ihA...
+    apply: ihm...
+    econstructor... }
+  { move=>Γ A B m n s tym ihm tyn ihn m0 ξ e. sta0_to_sta.
+    destruct m0; inv e.
+    have[s0 tyP]:=sta_valid tym.
+    have[t[tyB/sort_inj e]]:=sta_pi0_inv tyP. subst.
+    apply: sta_conv.
+    apply: sta_conv_beta.
+    apply: conv_sym.
+    apply: sta_cren_conv0...
+    econstructor...
+    have/=:=sta_subst tyB tyn... }
+  { move=>Γ A B m n s tym ihm tyn ihn m0 ξ e. sta0_to_sta.
+    destruct m0; inv e.
+    have[s0 tyP]:=sta_valid tym.
+    have[t[tyB/sort_inj e]]:=sta_pi1_inv tyP. subst.
+    apply: sta_conv.
+    apply: sta_conv_beta.
+    apply: conv_sym.
+    apply: sta_cren_conv0...
+    econstructor...
+    have/=:=sta_subst tyB tyn... }
+  { move=>Γ A B s r t ord tyA ihA tyB ihB m ξ e. sta0_to_sta.
+    destruct m; inv e.
+    econstructor...
+    apply: sta_ctx_conv.
+    apply: conv_sym.
+    apply: sta_cren_conv0...
+    eauto.
+    eauto. }
+  { move=>Γ A B s r t ord1 ord2 tyA ihA tyB ihB m ξ e. sta0_to_sta.
+    destruct m; inv e.
+    econstructor.
+    apply: ord1.
+    apply: ord2.
+    eauto.
+    apply: sta_ctx_conv.
+    apply: conv_sym.
+    apply: sta_cren_conv0...
+    eauto.
+    eauto. }
+  { move=>Γ A B m n t tyS ihS tym ihm tyn ihn m0 ξ e. sta0_to_sta.
+    destruct m0; inv e.
+    have[s[r[ord[tyA[tyB _]]]]]:=sta_sig0_inv tyS.
+    econstructor...
+    apply: sta_conv.
+    apply: sta_conv_beta.
+    apply: sta_cren_conv0...
+    eauto.
+    have:=sta_subst tyB (ihm _ _ erefl)... }
+  { move=>Γ A B m n t tyS ihS tym ihm tyn ihn m0 ξ e. sta0_to_sta.
+    destruct m0; inv e.
+    have[s[r[ord1[ord2[tyA[tyB _]]]]]]:=sta_sig1_inv tyS.
+    econstructor...
+    apply: sta_conv.
+    apply: sta_conv_beta.
+    apply: sta_cren_conv0...
+    eauto.
+    have:=sta_subst tyB (ihm _ _ erefl)... }
+  { move=>Γ A B C m n s t tyS ihS tym ihm tyn ihn m0 ξ e. sta0_to_sta.
+    destruct m0; inv e.
+    have wf:=sta_type_wf tyS. inv wf.
+    have[s1[r[ord[tyA[tyB/sort_inj e]]]]]:=sta_sig0_inv H2. subst.
+    have cs: term_csubst (m0 .: ids) (term_cren m0 ξ .: ids) ξ.
+    move=>[|x]...
+    erewrite<-(term_cren_subst _ cs).
+    have agr:sta_agree_subst (B :: A :: Γ) (Pair0 (Var 1) (Var 0) t .: ren (+2)) (Sig0 A B t :: Γ).
+    { econstructor.
+      replace (ren (+2)) with (ids >> (ren (+1)) >> (ren (+1))) by autosubst.
+      econstructor...
+      econstructor...
+      asimpl.
+      econstructor.
+      replace (Sig0 A.[ren (+2)] B.[ren (0 .: (+3))] t)
+        with (Sig0 A B t).[ren (+2)] by autosubst.
+      replace (Sort t) with (Sort t).[ren (+2)] by eauto.
+      apply: sta_rename...
+      replace (+2) with ((+1) >>> (+1) >>> id) by autosubst.
+      econstructor...
+      econstructor...
+      apply: sta_agree_ren_refl...
+      repeat constructor...
+      replace A.[ren (+2)] with A.[ren (+1)].[ren (+1)] by autosubst.
+      repeat constructor.
+      asimpl.
+      repeat constructor... }
+    apply: sta_conv.
+    apply: conv_sym.
+    apply: sta_cren_conv0...
+    econstructor...
+    2:{ have/=:=sta_subst tyS tym.
+        rewrite<-term_cren_beta1... }
+    apply: sta_conv.
+    apply: sta_conv_subst.
+    2:{ apply: ihn... }
+    apply: sta_cren_conv0...
+    have/=:=sta_substitution (ihS _ _ erefl) agr... }
+  { move=>Γ A B C m n s t tyS ihS tym ihm tyn ihn m0 ξ e. sta0_to_sta.
+    destruct m0; inv e.
+    have wf:=sta_type_wf tyS. inv wf.
+    have[s1[r[ord1[ord2[tyA[tyB/sort_inj e]]]]]]:=sta_sig1_inv H2. subst.
+    have cs: term_csubst (m0 .: ids) (term_cren m0 ξ .: ids) ξ.
+    move=>[|x]...
+    erewrite<-(term_cren_subst _ cs).
+    have agr:sta_agree_subst (B :: A :: Γ) (Pair1 (Var 1) (Var 0) t .: ren (+2)) (Sig1 A B t :: Γ).
+    { econstructor.
+      replace (ren (+2)) with (ids >> (ren (+1)) >> (ren (+1))) by autosubst.
+      econstructor...
+      econstructor...
+      asimpl.
+      econstructor.
+      replace (Sig1 A.[ren (+2)] B.[ren (0 .: (+3))] t)
+        with (Sig1 A B t).[ren (+2)] by autosubst.
+      replace (Sort t) with (Sort t).[ren (+2)] by eauto.
+      apply: sta_rename...
+      replace (+2) with ((+1) >>> (+1) >>> id) by autosubst.
+      econstructor...
+      econstructor...
+      apply: sta_agree_ren_refl...
+      repeat constructor...
+      replace A.[ren (+2)] with A.[ren (+1)].[ren (+1)] by autosubst.
+      repeat constructor.
+      asimpl.
+      repeat constructor... }
+    apply: sta_conv.
+    apply: conv_sym.
+    apply: sta_cren_conv0...
+    apply: sta_letin1...
+    2:{ have/=:=sta_subst tyS tym.
+        rewrite<-term_cren_beta1... }
+    apply: sta_conv.
+    apply: sta_conv_subst.
+    2:{ apply: ihn... }
+    apply: sta_cren_conv0...
+    have/=:=sta_substitution (ihS _ _ erefl) agr... }
+  { move=>Γ A m s tyA ihA tym ihm m0 ξ e. sta0_to_sta.
+    destruct m0; inv e.
+    apply: sta_conv.
+    apply: conv_sym.
+    apply: sta_cren_conv0...
+    constructor.
+    apply: sta_ctx_conv.
+    apply: conv_sym.
+    apply: sta_cren_conv0...
+    apply: ihA...
+    apply: sta_conv.
+    2:{ apply: ihm... }
+    apply: sta_conv_subst.
+    apply: sta_cren_conv0...
+    have/=:=sta_weaken (ihA _ _ erefl) tyA...
+    eauto. }
+  { move=>Γ A m n1 n2 s tyA ihA tym ihm tyn1 ihn1 tyn2 ihn2 m0 ξ e. sta0_to_sta.
+    destruct m0; inv e.
+    have wf:=sta_type_wf tyA. inv wf.
+    rewrite<-term_cren_beta1.
+    apply: sta_conv.
+    apply: conv_sym.
+    apply: sta_cren_conv0...
+    econstructor...
+    apply: sta_conv.
+    apply: sta_conv_subst.
+    apply: sta_cren_conv0...
+    apply: ihn1...
+    have:=sta_subst (ihA _ _ erefl) (sta_tt H1)...
+    apply: sta_conv.
+    apply: sta_conv_subst.
+    apply: sta_cren_conv0...
+    apply: ihn2...
+    have:=sta_subst (ihA _ _ erefl) (sta_ff H1)...
+    have/=:=sta_subst tyA tym.
+    rewrite<-term_cren_beta1... }
+  { move=>Γ r A B s tyA ihA tyB ihB m ξ e. sta0_to_sta.
+    destruct m; inv e.
+    constructor.
+    apply: sta_ctx_conv.
+    apply: conv_sym.
+    apply: sta_cren_conv0...
+    apply: ihA...
+    apply: ihB... }
+  { move=>Γ r A B s tyA ihA tyB ihB m ξ e. sta0_to_sta.
+    destruct m; inv e.
+    constructor.
+    apply: sta_ctx_conv.
+    apply: conv_sym.
+    apply: sta_cren_conv0...
+    apply: ihA...
+    apply: ihB... }
+  { move=>Γ A m s tyC ihC tym ihm m0 ξ e. sta0_to_sta.
+    destruct m0; inv e.
+    have tyC':=ihC (Ch true m0) ξ erefl.
+    have[tym0/sort_inj e]:=sta_ch_inv tyC. subst.
+    apply: sta_conv.
+    apply: sta_conv_io.
+    apply: sta_conv_ch.
+    apply: conv_sym.
+    apply: sta_cren_conv0...
+    econstructor.
+    apply: sta_ctx_conv.
+    3:{ apply: ihm... }
+    apply: sta_conv_ch.
+    apply: conv_sym.
+    apply: sta_cren_conv0...
+    eauto.
+    econstructor.
+    econstructor... }
 Qed.
